sf/Hoare.v
@@ -31,7 +31,7 @@ Require Export Imp.
         - correctness (in the sense of preserving meaning) of a number
           of useful program transformations
 
-        - behavioral equivalence of programs (in the [Equiv] chapter). 
+        - behavioral equivalence of programs (in the [Equiv] chapter).
 
     If we stopped here, we would already have something useful: a set
     of tools for defining and discussing programming languages and
@@ -66,7 +66,7 @@ Require Export Imp.
     systems. *)
 
 
-  
+
 (* ####################################################### *)
 (** * Hoare Logic *)
 
@@ -120,7 +120,7 @@ End ExAssertions.
     discussing examples informally, we'll adopt some simplifying
     conventions: we'll drop the initial [fun st =>], and we'll write
     just [X] to mean [st X].  Thus, instead of writing *)
-(** 
+(**
       fun st => (st Z) * (st Z) <= m /\
                 ~ ((S (st Z)) * (S (st Z)) <= m)
     we'll write just
@@ -195,12 +195,12 @@ Notation "{{ P }}  c  {{ Q }}" :=
 
    4) {{True}} c {{False}}
 
-   5) {{X = m}} 
+   5) {{X = m}}
       c
       {{Y = real_fact m}}.
 
-   6) {{True}} 
-      c 
+   6) {{True}}
+      c
       {{(Z * Z) <= m /\ ~ (((S Z) * (S Z)) <= m)}}
 
  *)
@@ -270,7 +270,7 @@ Proof.
   unfold not in H. apply H in HP.
   inversion HP.  Qed.
 
-(* ####################################################### *) 
+(* ####################################################### *)
 (** ** Proof Rules *)
 
 (** The goal of Hoare logic is to provide a _compositional_
@@ -284,7 +284,7 @@ Proof.
     together. We will prove programs correct using these proof rules,
     without ever unfolding the definition of [hoare_triple]. *)
 
-(* ####################################################### *) 
+(* ####################################################### *)
 (** *** Assignment *)
 
 (** The rule for assignment is the most fundamental of the Hoare logic
@@ -305,7 +305,7 @@ Proof.
 
     More generally, if [a] is _any_ arithmetic expression, then
        {{ a = 1 }}  X ::= a {{ X = 1 }}
-    is a valid Hoare triple. 
+    is a valid Hoare triple.
 
     This can be made even more general. To conclude that an
     _arbitrary_ property [Q] holds after [X ::= a], we need to assume
@@ -319,18 +319,18 @@ Proof.
     For example, these are valid applications of the assignment
     rule:
       {{ (X <= 5) [X |-> X + 1]
-         i.e., X + 1 <= 5 }}  
-      X ::= X + 1  
+         i.e., X + 1 <= 5 }}
+      X ::= X + 1
       {{ X <= 5 }}
 
       {{ (X = 3) [X |-> 3]
-         i.e., 3 = 3}}  
-      X ::= 3  
+         i.e., 3 = 3}}
+      X ::= 3
       {{ X = 3 }}
 
       {{ (0 <= X /\ X <= 5) [X |-> 3]
-         i.e., (0 <= 3 /\ 3 <= 5)}}  
-      X ::= 3  
+         i.e., (0 <= 3 /\ 3 <= 5)}}
+      X ::= 3
       {{ 0 <= X /\ X <= 5 }}
 *)
 
@@ -339,8 +339,8 @@ Proof.
     That is, given a proposition [P], a variable [X], and an
     arithmetic expression [a], we want to derive another proposition
     [P'] that is just the same as [P] except that, wherever [P]
-    mentions [X], [P'] should instead mention [a].  
-   
+    mentions [X], [P'] should instead mention [a].
+
     Since [P] is an arbitrary Coq proposition, we can't directly
     "edit" its text.  Instead, we can achieve the effect we want by
     evaluating [P] in an updated state: *)
@@ -358,38 +358,38 @@ Notation "P [ X |-> a ]" := (assn_sub X a P) (at level 10).
     To see how this works, let's calculate what happens with a couple
     of examples.  First, suppose [P'] is [(X <= 5) [X |-> 3]] -- that
     is, more formally, [P'] is the Coq expression
-    fun st => 
-      (fun st' => st' X <= 5) 
+    fun st =>
+      (fun st' => st' X <= 5)
       (update st X (aeval st (ANum 3))),
-    which simplifies to 
-    fun st => 
-      (fun st' => st' X <= 5) 
+    which simplifies to
+    fun st =>
+      (fun st' => st' X <= 5)
       (update st X 3)
     and further simplifies to
-    fun st => 
+    fun st =>
       ((update st X 3) X) <= 5)
     and by further simplification to
-    fun st => 
+    fun st =>
       (3 <= 5).
     That is, [P'] is the assertion that [3] is less than or equal to
     [5] (as expected).
 
     For a more interesting example, suppose [P'] is [(X <= 5) [X |->
     X+1]].  Formally, [P'] is the Coq expression
-    fun st => 
-      (fun st' => st' X <= 5) 
+    fun st =>
+      (fun st' => st' X <= 5)
       (update st X (aeval st (APlus (AId X) (ANum 1)))),
-    which simplifies to 
-    fun st => 
+    which simplifies to
+    fun st =>
       (((update st X (aeval st (APlus (AId X) (ANum 1))))) X) <= 5
     and further simplifies to
-    fun st => 
+    fun st =>
       (aeval st (APlus (AId X) (ANum 1))) <= 5.
     That is, [P'] is the assertion that [X+1] is at most [5].
 
 *)
 
-(** Now we can give the precise proof rule for assignment: 
+(** Now we can give the precise proof rule for assignment:
       ------------------------------ (hoare_asgn)
       {{Q [X |-> a]}} X ::= a {{Q}}
 *)
@@ -422,7 +422,7 @@ Proof.
     2) {{ (0 <= X /\ X <= 5) [X |-> 3] }}
        X ::= 3
        {{ 0 <= X /\ X <= 5 }}
-   ...into formal statements [assn_sub_ex1, assn_sub_ex2] 
+   ...into formal statements [assn_sub_ex1, assn_sub_ex2]
    and use [hoare_asgn] to prove them. *)
 
 (* FILL IN HERE *)
@@ -439,6 +439,20 @@ Proof.
     (informally). Hint: The rule universally quantifies over the
     arithmetic expression [a], and your counterexample needs to
     exhibit an [a] for which the rule doesn't work. *)
+Theorem hoare_asgn_wrong:
+  exists a, ~ {{ fun st => True }} X ::= a {{ fun st => st X = aeval st a}}.
+Proof.
+  exists (APlus (AId X) (ANum 1)).
+  intros not.
+  unfold beval, assn_sub, update, hoare_triple, assert_implies in not.
+  remember empty_state as st.
+  remember (update st X (st X + 1)) as st'.
+  assert ((X ::= (APlus (AId X) (ANum 1))) / st || st') as HH.
+
+  rewrite Heqst. rewrite Heqst'. subst. apply E_Ass. reflexivity.
+
+  subst. apply not in HH. inversion HH. auto.
+Qed.
 
 (* FILL IN HERE *)
 (** [] *)
@@ -468,7 +482,18 @@ Theorem hoare_asgn_fwd :
   {{fun st => P (update st X m) /\ st X = aeval (update st X m) a }}.
 Proof.
   intros functional_extensionality m a P.
-  (* FILL IN HERE *) Admitted.
+  unfold hoare_triple. intros st st' E Pre.
+    destruct Pre as [Pre1 Pre2].
+    inversion E; subst.
+    assert (st = update (update st X (aeval st a)) X (st X)) as Eq.
+      apply functional_extensionality. intros x.
+      rewrite update_shadow.
+      rewrite update_same; reflexivity.
+    rewrite <- Eq.
+    split.
+      assumption.
+      reflexivity.
+Qed.
 (** [] *)
 
 (** **** Exercise: 2 stars, advanced (hoare_asgn_fwd_exists)  *)
@@ -493,10 +518,12 @@ Theorem hoare_asgn_fwd_exists :
                 st X = aeval (update st X m) a }}.
 Proof.
   intros functional_extensionality a P.
+  unfold hoare_triple.
+  intros. inversion H. subst. exists (aeval st a). split. simpl. replace (update (update st X (aeval st a)) X (aeval st a)) with st. apply H0. apply functional_extensionality. intros. rewrite update_shadow.
   (* FILL IN HERE *) Admitted.
 (** [] *)
 
-(* ####################################################### *) 
+(* ####################################################### *)
 (** *** Consequence *)
 
 (** Sometimes the preconditions and postconditions we get from the
@@ -508,7 +535,7 @@ Proof.
 
     For instance, while
       {{(X = 3) [X |-> 3]}} X ::= 3 {{X = 3}},
-    follows directly from the assignment rule, 
+    follows directly from the assignment rule,
       {{True}} X ::= 3 {{X = 3}}.
     does not.  This triple is valid, but it is not an instance of
     [hoare_asgn] because [True] and [(X = 3) [X |-> 3]] are not
@@ -530,7 +557,7 @@ Proof.
                 {{P}} c {{Q}}
 
                 {{P}} c {{Q'}}
-                  Q' ->> Q 
+                  Q' ->> Q
          -----------------------------    (hoare_consequence_post)
                 {{P}} c {{Q}}
 *)
@@ -543,7 +570,7 @@ Theorem hoare_consequence_pre : forall (P P' Q : Assertion) c,
   {{P}} c {{Q}}.
 Proof.
   intros P P' Q c Hhoare Himp.
-  intros st st' Hc HP. apply (Hhoare st st'). 
+  intros st st' Hc HP. apply (Hhoare st st').
   assumption. apply Himp. assumption. Qed.
 
 Theorem hoare_consequence_post : forall (P Q Q' : Assertion) c,
@@ -552,17 +579,17 @@ Theorem hoare_consequence_post : forall (P Q Q' : Assertion) c,
   {{P}} c {{Q}}.
 Proof.
   intros P Q Q' c Hhoare Himp.
-  intros st st' Hc HP. 
+  intros st st' Hc HP.
   apply Himp.
-  apply (Hhoare st st'). 
+  apply (Hhoare st st').
   assumption. assumption. Qed.
 
 (** For example, we might use the first consequence rule like this:
                 {{ True }} ->>
-                {{ 1 = 1 }} 
+                {{ 1 = 1 }}
     X ::= 1
                 {{ X = 1 }}
-    Or, formally... 
+    Or, formally...
 *)
 
 Example hoare_asgn_example1 :
@@ -576,7 +603,7 @@ Qed.
 
 (** Finally, for convenience in some proofs, we can state a "combined"
     rule of consequence that allows us to vary both the precondition
-    and the postcondition. 
+    and the postcondition.
                 {{P'}} c {{Q'}}
                    P ->> P'
                    Q' ->> Q
@@ -616,8 +643,8 @@ Proof.
     going to be filled in soon." *)
 
 Example hoare_asgn_example1' :
-  {{fun st => True}} 
-  (X ::= (ANum 1)) 
+  {{fun st => True}}
+  (X ::= (ANum 1))
   {{fun st => st X = 1}}.
 Proof.
   eapply hoare_consequence_pre.
@@ -651,8 +678,8 @@ Proof.
      ?171 : [P : nat -> nat -> Prop
              Q : nat -> Prop
              HP : forall x y : nat, P x y
-             HQ : forall x y : nat, P x y -> Q x |- nat] 
-  
+             HQ : forall x y : nat, P x y -> Q x |- nat]
+
      (dependent evars: ?171 open,)
 
      You can use Grab Existential Variables.
@@ -709,13 +736,13 @@ Proof.
   intros P Q HP HQ. destruct HP as [y HP']. eapply HQ. eassumption.
 Qed.
 
-    
+
 
 (** **** Exercise: 2 stars (hoare_asgn_examples_2)  *)
 (** Translate these informal Hoare triples...
        {{ X + 1 <= 5 }}  X ::= X + 1  {{ X <= 5 }}
        {{ 0 <= 3 /\ 3 <= 5 }}  X ::= 3  {{ 0 <= X /\ X <= 5 }}
-   ...into formal statements [assn_sub_ex1', assn_sub_ex2'] and 
+   ...into formal statements [assn_sub_ex1', assn_sub_ex2'] and
    use [hoare_asgn] and [hoare_consequence_pre] to prove them. *)
 
 (* FILL IN HERE *)
@@ -736,7 +763,7 @@ Proof.
   intros P st st' H HP. inversion H. subst.
   assumption.  Qed.
 
-(* ####################################################### *) 
+(* ####################################################### *)
 (** *** Sequencing *)
 
 (** More interestingly, if the command [c1] takes any state where
@@ -744,7 +771,7 @@ Proof.
     state where [Q] holds to one where [R] holds, then doing [c1]
     followed by [c2] will take any state where [P] holds to one
     where [R] holds:
-        {{ P }} c1 {{ Q }} 
+        {{ P }} c1 {{ Q }}
         {{ Q }} c2 {{ R }}
        ---------------------  (hoare_seq)
        {{ P }} c1;;c2 {{ R }}
@@ -779,15 +806,15 @@ Proof.
 *)
 
 Example hoare_asgn_example3 : forall a n,
-  {{fun st => aeval st a = n}} 
-  (X ::= a;; SKIP) 
+  {{fun st => aeval st a = n}}
+  (X ::= a;; SKIP)
   {{fun st => st X = n}}.
 Proof.
   intros a n. eapply hoare_seq.
   Case "right part of seq".
     apply hoare_skip.
   Case "left part of seq".
-    eapply hoare_consequence_pre. apply hoare_asgn. 
+    eapply hoare_consequence_pre. apply hoare_asgn.
     intros st H. subst. reflexivity. Qed.
 
 (** You will most often use [hoare_seq] and
@@ -806,10 +833,12 @@ Proof.
 *)
 
 Example hoare_asgn_example4 :
-  {{fun st => True}} (X ::= (ANum 1);; Y ::= (ANum 2)) 
+  {{fun st => True}} (X ::= (ANum 1);; Y ::= (ANum 2))
   {{fun st => st X = 1 /\ st Y = 2}}.
 Proof.
-  (* FILL IN HERE *) Admitted.
+  intros. eapply hoare_seq. apply hoare_asgn. eapply hoare_consequence_pre. eapply hoare_asgn.
+  unfold assn_sub, update, assert_implies. simpl. intros. auto.
+Qed.
 (** [] *)
 
 (** **** Exercise: 3 stars (swap_exercise)  *)
@@ -823,7 +852,7 @@ Definition swap_program : com :=
   (* FILL IN HERE *) admit.
 
 Theorem swap_exercise :
-  {{fun st => st X <= st Y}} 
+  {{fun st => st X <= st Y}}
   swap_program
   {{fun st => st Y <= st X}}.
 Proof.
@@ -841,7 +870,7 @@ Proof.
 (* FILL IN HERE *)
 (** [] *)
 
-(* ####################################################### *) 
+(* ####################################################### *)
 (** *** Conditionals *)
 
 (** What sort of rule do we want for reasoning about conditional
@@ -854,15 +883,15 @@ Proof.
       {{P}} IFB b THEN c1 ELSE c2 {{Q}}
    However, this is rather weak. For example, using this rule,
    we cannot show that:
-     {{ True }} 
+     {{ True }}
      IFB X == 0
      THEN Y ::= 2
-     ELSE Y ::= X + 1 
+     ELSE Y ::= X + 1
      FI
      {{ X <= Y }}
    since the rule tells us nothing about the state in which the
    assignments take place in the "then" and "else" branches. *)
-   
+
 (** But we can actually say something more precise.  In the
    "then" branch, we know that the boolean expression [b] evaluates to
    [true], and in the "else" branch, we know it evaluates to [false].
@@ -874,7 +903,7 @@ Proof.
               {{P /\  b}} c1 {{Q}}
               {{P /\ ~b}} c2 {{Q}}
       ------------------------------------  (hoare_if)
-      {{P}} IFB b THEN c1 ELSE c2 FI {{Q}} 
+      {{P}} IFB b THEN c1 ELSE c2 FI {{Q}}
 *)
 
 (** To interpret this rule formally, we need to do a little work.
@@ -912,24 +941,24 @@ Theorem hoare_if : forall P Q b c1 c2,
   {{P}} (IFB b THEN c1 ELSE c2 FI) {{Q}}.
 Proof.
   intros P Q b c1 c2 HTrue HFalse st st' HE HP.
-  inversion HE; subst. 
+  inversion HE; subst.
   Case "b is true".
-    apply (HTrue st st'). 
-      assumption. 
-      split. assumption. 
+    apply (HTrue st st').
+      assumption.
+      split. assumption.
              apply bexp_eval_true. assumption.
   Case "b is false".
-    apply (HFalse st st'). 
-      assumption. 
+    apply (HFalse st st').
+      assumption.
       split. assumption.
              apply bexp_eval_false. assumption. Qed.
 
 
-(* ####################################################### *) 
+(* ####################################################### *)
 
 (** * Hoare Logic: So Far *)
 
-(** 
+(**
 Idea: create a _domain specific logic_ for reasoning about properties of Imp programs.
 
 - This hides the low-level details of the semantics of the program
@@ -938,7 +967,7 @@ Idea: create a _domain specific logic_ for reasoning about properties of Imp pro
 
 The basic structure is given by _Hoare triples_ of the form:
   {{P}} c {{Q}}
-]] 
+]]
 
 - [P] and [Q] are predicates about the state of the Imp program
 - "If command [c] is started in a state satisfying assertion
@@ -957,7 +986,7 @@ The basic structure is given by _Hoare triples_ of the form:
              --------------------  (hoare_skip)
              {{ P }} SKIP {{ P }}
 
-               {{ P }} c1 {{ Q }} 
+               {{ P }} c1 {{ Q }}
                {{ Q }} c2 {{ R }}
               ---------------------  (hoare_seq)
               {{ P }} c1;;c2 {{ R }}
@@ -965,7 +994,7 @@ The basic structure is given by _Hoare triples_ of the form:
               {{P /\  b}} c1 {{Q}}
               {{P /\ ~b}} c2 {{Q}}
       ------------------------------------  (hoare_if)
-      {{P}} IFB b THEN c1 ELSE c2 FI {{Q}} 
+      {{P}} IFB b THEN c1 ELSE c2 FI {{Q}}
 
 
                 {{P'}} c {{Q'}}
@@ -980,11 +1009,11 @@ The basic structure is given by _Hoare triples_ of the form:
 (** Here is a formal proof that the program we used to motivate the
     rule satisfies the specification we gave. *)
 
-Example if_example : 
-    {{fun st => True}} 
-  IFB (BEq (AId X) (ANum 0)) 
-    THEN (Y ::= (ANum 2)) 
-    ELSE (Y ::= APlus (AId X) (ANum 1)) 
+Example if_example :
+    {{fun st => True}}
+  IFB (BEq (AId X) (ANum 0))
+    THEN (Y ::= (ANum 2))
+    ELSE (Y ::= APlus (AId X) (ANum 1))
   FI
     {{fun st => st X <= st Y}}.
 Proof.
@@ -1011,9 +1040,15 @@ Theorem if_minus_plus :
     THEN (Z ::= AMinus (AId Y) (AId X))
     ELSE (Y ::= APlus (AId X) (AId Z))
   FI
-  {{fun st => st Y = st X + st Z}}. 
+  {{fun st => st Y = st X + st Z}}.
 Proof.
-  (* FILL IN HERE *) Admitted.
+  eapply hoare_if.
+  intros st st'. intros.
+  inversion H. subst. simpl. destruct H0. unfold update. simpl. inversion H1. apply le_plus_minus. apply ble_nat_true. apply H3.
+
+  intros st st'. intros.
+  inversion H. subst. destruct H0. simpl. unfold update. simpl. reflexivity.
+Qed.
 
 (* ####################################################### *)
 (** *** Exercise: One-sided conditionals *)
@@ -1050,17 +1085,17 @@ Tactic Notation "com_cases" tactic(first) ident(c) :=
   [ Case_aux c "SKIP" | Case_aux c "::=" | Case_aux c ";"
   | Case_aux c "IFB" | Case_aux c "WHILE" | Case_aux c "CIF1" ].
 
-Notation "'SKIP'" := 
+Notation "'SKIP'" :=
   CSkip.
-Notation "c1 ;; c2" := 
+Notation "c1 ;; c2" :=
   (CSeq c1 c2) (at level 80, right associativity).
-Notation "X '::=' a" := 
+Notation "X '::=' a" :=
   (CAss X a) (at level 60).
-Notation "'WHILE' b 'DO' c 'END'" := 
+Notation "'WHILE' b 'DO' c 'END'" :=
   (CWhile b c) (at level 80, right associativity).
-Notation "'IFB' e1 'THEN' e2 'ELSE' e3 'FI'" := 
+Notation "'IFB' e1 'THEN' e2 'ELSE' e3 'FI'" :=
   (CIf e1 e2 e3) (at level 80, right associativity).
-Notation "'IF1' b 'THEN' c 'FI'" := 
+Notation "'IF1' b 'THEN' c 'FI'" :=
   (CIf1 b c) (at level 80, right associativity).
 
 (** Next we need to extend the evaluation relation to accommodate
@@ -1103,13 +1138,13 @@ Tactic Notation "ceval_cases" tactic(first) ident(c) :=
 (** Now we repeat (verbatim) the definition and notation of Hoare triples. *)
 
 Definition hoare_triple (P:Assertion) (c:com) (Q:Assertion) : Prop :=
-  forall st st', 
+  forall st st',
        c / st || st'  ->
        P st  ->
        Q st'.
 
-Notation "{{ P }}  c  {{ Q }}" := (hoare_triple P c Q) 
-                                  (at level 90, c at next level) 
+Notation "{{ P }}  c  {{ Q }}" := (hoare_triple P c Q)
+                                  (at level 90, c at next level)
                                   : hoare_spec_scope.
 
 (** Finally, we (i.e., you) need to state and prove a theorem,
@@ -1117,9 +1152,17 @@ Notation "{{ P }}  c  {{ Q }}" := (hoare_triple P c Q)
     for one-sided conditionals. Try to come up with a rule that is
     both sound and as precise as possible. *)
 
+Theorem hoare_if1 : forall P Q b c1,
+  {{fun st => P st /\ bassn b st}} c1 {{Q}} ->
+  {{fun st => P st /\ ~(bassn b st)}} SKIP {{Q}} ->
+  {{P}} (IF1 b THEN c1 FI) {{Q}}.
+Proof.
+  intros P Q b c1 HTrue HFalse st st' HE HP.
+  inversion HE; subst.
+Qed.
 (* FILL IN HERE *)
 
-(** For full credit, prove formally [hoare_if1_good] that your rule is 
+(** For full credit, prove formally [hoare_if1_good] that your rule is
     precise enough to show the following valid Hoare triple:
   {{ X + Y = Z }}
   IF1 Y <> 0 THEN
@@ -1139,7 +1182,11 @@ Lemma hoare_if1_good :
     X ::= APlus (AId X) (AId Y)
   FI
   {{ fun st => st X = st Z }}.
-Proof. (* FILL IN HERE *) Admitted.
+Proof.
+  eapply hoare_if1.
+  intros st st'. intros. inversion H. subst. unfold update. simpl. destruct H0. apply H0.
+  intros st st'. intros. inversion H; subst. destruct H0. unfold bassn in H1. simpl in H1. SearchAbout negb. apply eq_true_negb_classical in H1. apply beq_nat_true_iff in H1. rewrite H1 in H0. omega.
+Qed.
 
 End If1.
 (** [] *)
@@ -1153,7 +1200,7 @@ End If1.
       WHILE b DO c END
     and we want to find a pre-condition [P] and a post-condition
     [Q] such that
-      {{P}} WHILE b DO c END {{Q}} 
+      {{P}} WHILE b DO c END {{Q}}
     is a valid triple. *)
 
 (** *** *)
@@ -1167,17 +1214,17 @@ End If1.
       {{P}} WHILE b DO c END {{P}}.
 *)
 
-(** 
+(**
     But, as we remarked above for the conditional, we know a
     little more at the end -- not just [P], but also the fact
     that [b] is false in the current state.  So we can enrich the
     postcondition a little:
 *)
-(** 
+(**
       {{P}} WHILE b DO c END {{P /\ ~b}}
 *)
 
-(** 
+(**
     What about the case where the loop body _does_ get executed?
     In order to ensure that [P] holds when the loop finally
     exits, we certainly need to make sure that the command [c]
@@ -1188,12 +1235,12 @@ End If1.
     that [P] holds at the beginning of [c].  This leads us to the
     following rule:
 *)
-(** 
+(**
                    {{P}} c {{P}}
-        -----------------------------------  
+        -----------------------------------
         {{P}} WHILE b DO c END {{P /\ ~b}}
 *)
-(** 
+(**
     This is almost the rule we want, but again it can be improved a
     little: at the beginning of the loop body, we know not only that
     [P] holds, but also that the guard [b] is true in the current
@@ -1213,8 +1260,8 @@ Lemma hoare_while : forall P b c,
   {{P}} WHILE b DO c END {{fun st => P st /\ ~ (bassn b st)}}.
 Proof.
   intros P b c Hhoare st st' He HP.
-  (* Like we've seen before, we need to reason by induction 
-     on [He], because, in the "keep looping" case, its hypotheses 
+  (* Like we've seen before, we need to reason by induction
+     on [He], because, in the "keep looping" case, its hypotheses
      talk about the whole loop instead of just [c]. *)
   remember (WHILE b DO c END) as wcom eqn:Heqwcom.
   ceval_cases (induction He) Case;
@@ -1253,16 +1300,16 @@ Example while_example :
   DO X ::= APlus (AId X) (ANum 1) END
     {{fun st => st X = 3}}.
 Proof.
-  eapply hoare_consequence_post. 
-  apply hoare_while. 
-  eapply hoare_consequence_pre. 
-  apply hoare_asgn. 
+  eapply hoare_consequence_post.
+  apply hoare_while.
+  eapply hoare_consequence_pre.
+  apply hoare_asgn.
   unfold bassn, assn_sub, assert_implies, update. simpl.
     intros st [H1 H2]. apply ble_nat_true in H2. omega.
-  unfold bassn, assert_implies. intros st [Hle Hb]. 
-    simpl in Hb. destruct (ble_nat (st X) 2) eqn : Heqle. 
-    apply ex_falso_quodlibet. apply Hb; reflexivity.  
-    apply ble_nat_false in Heqle. omega. 
+  unfold bassn, assert_implies. intros st [Hle Hb].
+    simpl in Hb. destruct (ble_nat (st X) 2) eqn : Heqle.
+    apply ex_falso_quodlibet. apply Hb; reflexivity.
+    apply ble_nat_false in Heqle. omega.
 Qed.
 
 
@@ -1283,7 +1330,7 @@ Proof.
   eapply hoare_consequence_post.
   apply hoare_while.
   Case "Loop body preserves invariant".
-    apply hoare_post_true. intros st. apply I. 
+    apply hoare_post_true. intros st. apply I.
   Case "Loop invariant and negated guard imply postcondition".
     simpl. intros st [Hinv Hguard].
     apply ex_falso_quodlibet. apply Hguard. reflexivity.
@@ -1332,17 +1379,17 @@ Tactic Notation "com_cases" tactic(first) ident(c) :=
   | Case_aux c "IFB" | Case_aux c "WHILE"
   | Case_aux c "CRepeat" ].
 
-Notation "'SKIP'" := 
+Notation "'SKIP'" :=
   CSkip.
-Notation "c1 ;; c2" := 
+Notation "c1 ;; c2" :=
   (CSeq c1 c2) (at level 80, right associativity).
-Notation "X '::=' a" := 
+Notation "X '::=' a" :=
   (CAsgn X a) (at level 60).
-Notation "'WHILE' b 'DO' c 'END'" := 
+Notation "'WHILE' b 'DO' c 'END'" :=
   (CWhile b c) (at level 80, right associativity).
-Notation "'IFB' e1 'THEN' e2 'ELSE' e3 'FI'" := 
+Notation "'IFB' e1 'THEN' e2 'ELSE' e3 'FI'" :=
   (CIf e1 e2 e3) (at level 80, right associativity).
-Notation "'REPEAT' e1 'UNTIL' b2 'END'" := 
+Notation "'REPEAT' e1 'UNTIL' b2 'END'" :=
   (CRepeat e1 b2) (at level 80, right associativity).
 
 (** Add new rules for [REPEAT] to [ceval] below.  You can use the rules
@@ -1385,17 +1432,17 @@ Tactic Notation "ceval_cases" tactic(first) ident(c) :=
   [ Case_aux c "E_Skip" | Case_aux c "E_Ass"
   | Case_aux c "E_Seq"
   | Case_aux c "E_IfTrue" | Case_aux c "E_IfFalse"
-  | Case_aux c "E_WhileEnd" | Case_aux c "E_WhileLoop" 
+  | Case_aux c "E_WhileEnd" | Case_aux c "E_WhileLoop"
 (* FILL IN HERE *)
 ].
 
 (** A couple of definitions from above, copied here so they use the
     new [ceval]. *)
 
-Notation "c1 '/' st '||' st'" := (ceval st c1 st') 
+Notation "c1 '/' st '||' st'" := (ceval st c1 st')
                                  (at level 40, st at level 39).
 
-Definition hoare_triple (P:Assertion) (c:com) (Q:Assertion) 
+Definition hoare_triple (P:Assertion) (c:com) (Q:Assertion)
                         : Prop :=
   forall st st', (c / st || st') -> P st -> Q st'.
 
@@ -1516,8 +1563,8 @@ Tactic Notation "ceval_cases" tactic(first) ident(c) :=
 Definition hoare_triple (P:Assertion) (c:com) (Q:Assertion) : Prop :=
   forall st st', c / st || st' -> P st -> Q st'.
 
-Notation "{{ P }}  c  {{ Q }}" := (hoare_triple P c Q) 
-                                  (at level 90, c at next level) 
+Notation "{{ P }}  c  {{ Q }}" := (hoare_triple P c Q)
+                                  (at level 90, c at next level)
                                   : hoare_spec_scope.
 
 (** Complete the Hoare rule for [HAVOC] commands below by defining
@@ -1550,7 +1597,7 @@ End Himp.
              --------------------  (hoare_skip)
              {{ P }} SKIP {{ P }}
 
-               {{ P }} c1 {{ Q }} 
+               {{ P }} c1 {{ Q }}
                {{ Q }} c2 {{ R }}
               ---------------------  (hoare_seq)
               {{ P }} c1;;c2 {{ R }}
@@ -1558,7 +1605,7 @@ End Himp.
               {{P /\  b}} c1 {{Q}}
               {{P /\ ~b}} c2 {{Q}}
       ------------------------------------  (hoare_if)
-      {{P}} IFB b THEN c1 ELSE c2 FI {{Q}} 
+      {{P}} IFB b THEN c1 ELSE c2 FI {{Q}}
 
                {{P /\ b}} c {{P}}
         -----------------------------------  (hoare_while)
